substitution.v
@@ -1215,7 +1215,7 @@ with change_bvars_alphabt {NVar VarClass : Type} `{VarType NVar VarClass}  {gts 
 match bt with
 | bterm blv bnt => 
     let bnt' := @change_bvars_alpha NVar _ _ _ _  lv bnt in
-    let lvn := (freshVars (length blv) (option_map varClass (head blv)) (lv++(all_vars bnt')) blv) in
+    let lvn := freshReplacements blv (lv++(all_vars bnt')) in
          bterm lvn (ssubst_aux bnt' (var_ren blv lvn))
 end.
 
